- More Proofs

ImpCEvalFun_psp.v
@@ -2,4 +2,184 @@ Require Import Coq.omega.Omega.
 Require Import Coq.Arith.Arith.
 Require Import Imp Maps.
 
-±Fixpoint ceval_step
+Fixpoint ceval_step2 (st : state) (c : com) (i : nat) : state :=
+  match i with
+  | O => { --> 0 }
+  | S i' =>
+    match c with
+    | SKIP =>
+        st
+    | l ::= a1 =>
+        st & { l --> (aeval st a1) }
+    | c1 ;; c2 =>
+        let st' := ceval_step2 st c1 i' in
+        ceval_step2 st' c2 i'
+    | IFB b THEN c1 ELSE c2 FI =>
+        if (beval st b)
+          then ceval_step2 st c1 i'
+          else ceval_step2 st c2 i'
+    | WHILE b1 DO c1 END =>
+        if (beval st b1)
+        then let st' := ceval_step2 st c1 i' in
+            ceval_step2 st' c i'
+        else st
+    end
+  end.
+
+Fixpoint ceval_step3 (st : state) (c : com) (i : nat) : option state :=
+  match i with
+  | O => None
+  | S i' =>
+      match c with
+      | SKIP =>
+          Some st
+      | l ::= a1 =>
+          Some (st & { l --> (aeval st a1) })
+      | c1 ;; c2 =>
+          match (ceval_step3 st c1 i') with
+          | Some st' => ceval_step3 st' c2 i'
+          | None => None
+          end
+      | IFB b THEN c1 ELSE c2 FI =>
+          if (beval st b)
+            then ceval_step3 st c1 i'
+            else ceval_step3 st c2 i'
+      | WHILE b1 DO c1 END =>
+          if (beval st b1)
+          then match (ceval_step3 st c1 i') with
+               | Some st' => ceval_step3 st' c i'
+               | None => None
+               end
+          else Some st
+      end
+ end.
+
+Notation "'LETOPT' x <== e1 'IN' e2"
+  := (match e1 with
+      | Some x => e2
+      | None => None
+      end)
+  (right associativity, at level 60).
+
+Fixpoint ceval_step (st : state) (c : com) (i : nat) : option state :=
+  match i with
+  | O => None     
+  | S i' =>
+    match c with
+    | SKIP =>
+        Some st
+    | l ::= a1 =>
+        Some (st & { l --> (aeval st a1)})
+    | c1 ;; c2 =>
+        LETOPT st' <== ceval_step st c1 i' IN
+        ceval_step st' c2 i'
+    | IFB b THEN c1 ELSE c2 FI =>
+        if (beval st b)
+          then ceval_step st c1 i'
+          else ceval_step st c2 i'
+    | WHILE b1 DO c1 END =>
+        if (beval st b1)
+          then LETOPT st' <== ceval_step st c1 i' IN
+              ceval_step st' c i'
+          else Some st
+    end
+  end.
+
+Definition test_ceval (st:state) (c:com) :=
+  match ceval_step st c 500 with
+  | None => None
+  | Some st => Some (st X, st Y, st Z)
+  end.
+
+Compute
+  (test_ceval { --> 0}
+      (X ::= 2;;
+       IFB (X <= 1)
+          THEN Y ::= 3
+          ELSE Z ::= 4
+       FI)).
+
+(* Exercise: 2 stars, recommended (pup_to_n) *)
+
+Definition pup_to_n : com :=
+  (WHILE (1 <= X) DO
+    Y ::= Y + X;;
+    X ::= X - 1
+  END).
+
+(* Compute test_ceval {X --> 5} pup_to_n. *)
+
+Example pup_to_n_1 :
+  test_ceval {X --> 5} pup_to_n
+  = Some (0, 15, 0).
+Proof. reflexivity. Qed.
+
+(* Exercise: 2 stars, optional (peven) *)
+Definition peven : com :=
+  (WHILE (2 <= X) DO
+    X ::= X - 2;;
+    Z ::= X
+   END).
+
+(* Compute test_ceval {X --> 10} peven. *)
+
+Example peven_1 :
+  test_ceval {X --> 8} peven
+  = Some (0, 0, 0).
+Proof.
+  reflexivity.
+Qed.
+
+Example peven_2 :
+  test_ceval {X --> 81} peven
+  = Some (1, 0, 1).
+Proof.
+  reflexivity.
+Qed.
+
+(* Relational vs. Step-Indexed Evaluation *)
+Theorem ceval_step_ceval : forall c st st',
+  (exists i, ceval_step st c i = Some st') ->
+  c / st \\ st'.
+Proof.
+  intros c st st' H.
+  inversion H as [i E].
+  clear H.
+  generalize dependent st'.
+  generalize dependent st.
+  generalize dependent c.
+  induction i as [| i'].
+  - (* i = 0 *) intros c st st' H. inversion H.
+  - (* i = S i' *) intros c st st' H. 
+      destruct c;
+        simpl in H; inversion H; subst; clear H.
+    + (* c = SKIP *) apply E_Skip.
+    + (* c = ::= *) apply E_Ass. reflexivity.
+    + (* c = ;; *) destruct (ceval_step st c1 i') eqn:Heqr1.
+      * apply E_Seq with s;
+          try (apply IHi'; assumption).
+      * inversion H1.
+    + (* c = IF *) destruct (beval st b) eqn:Heqr1.
+      * (* b = true *) apply E_IfTrue.
+        { - assumption. }
+        { - apply IHi'. assumption. }
+      * (* b = false *) apply E_IfFalse.
+        { - assumption. }
+        { - apply IHi'. assumption. }
+     + (* c = WHILE *) destruct (beval st b) eqn:Heqr1.
+      { - (* b = true *) destruct (ceval_step st c i') eqn:Heqr2.
+          + apply E_WhileTrue with s;
+              try (assumption);
+              try (apply IHi'; assumption).
+          + apply E_WhileTrue with st';
+              try (assumption);
+              try (inversion H1). }
+       { - (* b = false *) inversion H1; subst. apply E_WhileFalse; assumption. }
+Qed.
+
+
+
+
+
+
+
